Added composition of taylor models.

Taylor_Models.thy
@@ -358,178 +358,22 @@ proof-
     by (induction p, simp_all)
 qed
 
-(* Operations on taylor models. *)
-fun TMNeg :: "taylor_model \<Rightarrow> taylor_model"
-where "TMNeg (TaylorModel p i) = TaylorModel (poly.Neg p) (-i)"
+(* Taylor models for basic functions. *)
 
-fun TMAdd :: "taylor_model \<Rightarrow> taylor_model \<Rightarrow> taylor_model"
-where "TMAdd (TaylorModel p1 i1) (TaylorModel p2 i2) = TaylorModel (poly.Add p1 p2) (i1+i2)"
+fun tm_const :: "float \<Rightarrow> taylor_model"
+where "tm_const c = TaylorModel (poly.C c) (Ivl 0 0)"
 
-fun TMSub :: "taylor_model \<Rightarrow> taylor_model \<Rightarrow> taylor_model"
-where "TMSub t1 t2 = TMAdd t1 (TMNeg t2)"
+fun tm_id :: "nat \<Rightarrow> taylor_model"
+where "tm_id n = TaylorModel (poly.Bound n) (Ivl 0 0)"
 
-(* TODO: Currently, this increases the degree of the polynomial! *)
-fun TMMul :: "taylor_model \<Rightarrow> taylor_model \<Rightarrow> float interval list \<Rightarrow> taylor_model"
-where "TMMul (TaylorModel p1 i1) (TaylorModel p2 i2) I = (
-  let d1=Ipoly I p1;
-      d2=Ipoly I p2
-  in TaylorModel (poly.Mul p1 p2) (i1*d2 + d1*i2 + i1*i2))"
-
-(* Validity of is preserved under taylor model arithmetic. *)
-lemma TMNeg_valid:
-assumes "valid_tm I f t"
-shows "valid_tm I (-f) (TMNeg t)"
-proof-
-  from valid_tmD[OF assms]
-  obtain p l u where t_def: 
-    "t = TaylorModel p (Ivl l u)"
-    "valid_ivl (Ivl l u)"
-    "num_params p \<le> length I"
-    "\<And>x. length x = length I \<Longrightarrow> (\<And>n. n < length I \<Longrightarrow> x ! n \<in> set_of (interval_map real (I ! n))) \<Longrightarrow> f x - Ipoly x p \<in> {l..u}"
-      by blast
-  show ?thesis
-    apply(rule)
-    apply(simp add: t_def(1) uminus_interval_def)
-    using t_def(2)
-    apply(simp)
-    apply(simp add: t_def(3))
-    proof-
-      fix x assume assms: "length x = length I" "(\<And>n. n < length I \<Longrightarrow> x ! n \<in> set_of (interval_map real (I ! n)))"
-      show "(-f) x - Ipoly x (Neg p) \<in> {(-u)..(-l)}"
-        using t_def(4)[OF assms] by simp
-    qed
-qed
-
-lemma TMAdd_valid:
-assumes "valid_tm I f t1"
-assumes "valid_tm I g t2"
-shows "valid_tm I (f + g) (TMAdd t1 t2)"
-proof-
-  from valid_tmD[OF assms(1)]
-  obtain p1 l1 u1 where t1_def:
-    "t1 = TaylorModel p1 (Ivl l1 u1)"
-    "valid_ivl (Ivl l1 u1)"
-    "num_params p1 \<le> length I"
-    "\<And>x. length x = length I \<Longrightarrow> (\<And>n. n < length I \<Longrightarrow> x ! n \<in> set_of (interval_map real (I ! n))) \<Longrightarrow> f x - Ipoly x p1 \<in> {l1..u1}"
-      by blast
-  from valid_tmD[OF assms(2)]
-  obtain p2 l2 u2 where t2_def:
-    "t2 = TaylorModel p2 (Ivl l2 u2)"
-    "valid_ivl (Ivl l2 u2)"
-    "num_params p2 \<le> length I"
-    "\<And>x. length x = length I \<Longrightarrow> (\<And>n. n < length I \<Longrightarrow> x ! n \<in> set_of (interval_map real (I ! n))) \<Longrightarrow> g x - Ipoly x p2 \<in> {l2..u2}"
-      by blast
-   
-  show "valid_tm I (f + g) (TMAdd t1 t2)"
-    proof(rule)
-      show "num_params (poly.Add p1 p2) \<le> length I"
-      by (simp add: t1_def(3) t2_def(3))
-    next
-      fix x assume assms: "length x = length I" "(\<And>n. n < length I \<Longrightarrow> x ! n \<in> set_of (interval_map real (I ! n)))"
-      from t1_def(4)[OF this] t2_def(4)[OF this]
-       show "(f + g) x - Ipoly x (poly.Add p1 p2) \<in> {(l1+l2)..(u1+u2)}"
-        by simp
-    next
-      show "valid_ivl (Ivl (l1 + l2) (u1 + u2))"
-        using t1_def(2) t2_def(2)
-        by simp
-    qed (simp add: t1_def(1) t2_def(1) plus_interval_def)
-qed
-
-lemma TMSub_valid:
-assumes "valid_tm I f t1"
-assumes "valid_tm I g t2"
-shows "valid_tm I (f - g) (TMSub t1 t2)"
-using TMAdd_valid[OF assms(1) TMNeg_valid[OF assms(2)]]
+lemma tm_const_valid:
+shows "valid_tm I (interpret_floatarith (Num c)) (tm_const c)"
 by simp
 
-(* TODO: Clean this proof up! *)
-lemma TMMul_valid:
-assumes "valid_tm I f t1"
-assumes "valid_tm I g t2"
-assumes "\<And>n. n < length I \<Longrightarrow> valid_ivl (I ! n)"
-shows "valid_tm I (f * g) (TMMul t1 t2 I)"
-proof-
-  from valid_tmD'[OF assms(1)]
-  obtain p1 i1 where t1_def:
-    "t1 = TaylorModel p1 i1"
-    "valid_ivl i1"
-    "num_params p1 \<le> length I"
-    "\<And>x. length x = length I \<Longrightarrow> (\<And>n. n < length I \<Longrightarrow> x ! n \<in> set_of (interval_map real (I ! n))) \<Longrightarrow> f x - Ipoly x p1 \<in> set_of i1"
-      by blast
-  from valid_tmD'[OF assms(2)]
-  obtain p2 i2 where t2_def:
-    "t2 = TaylorModel p2 i2"
-    "valid_ivl i2"
-    "num_params p2 \<le> length I"
-    "\<And>x. length x = length I \<Longrightarrow> (\<And>n. n < length I \<Longrightarrow> x ! n \<in> set_of (interval_map real (I ! n))) \<Longrightarrow> g x - Ipoly x p2 \<in> set_of i2"
-      by blast
-        
-  have v1: "valid_ivl (Ipoly I (poly_map interval_of p1))"
-    by (rule valid_ivl_Ipoly[OF t1_def(3) assms(3)])
-  have v2: "valid_ivl (Ipoly I (poly_map interval_of p2))"
-    by (rule valid_ivl_Ipoly[OF t2_def(3) assms(3)])
-      
-  show "valid_tm I (f * g) (TMMul t1 t2 I)"
-    unfolding t1_def t2_def TMMul.simps Let_def
-    apply(rule valid_tmI')
-    unfolding taylor_model.inject
-    apply(rule conjI[OF refl refl])
-    defer
-    using t1_def(3) t2_def(3)
-    apply(simp)
-    proof(goals)
-      case (1 x)
-      
-      obtain d1 :: real where d1_def: "d1 \<in> set_of i1" "f x - Ipoly x p1 = d1"
-        using t1_def(4)[OF 1] by auto
-      obtain d2 :: real where d2_def: "d2 \<in> set_of i2" "g x - Ipoly x p2 = d2"
-        using t2_def(4)[OF 1] by auto
-        
-      have a1: "length x = length (map (interval_map real) I)"
-        using 1(1) by simp
-      have a2: "num_params (poly_map real p1) \<le> length (map (interval_map real) I)"
-        using t1_def(3) by simp
-      have a2': "num_params (poly_map real p2) \<le> length (map (interval_map real) I)"
-        using t2_def(3) by simp
-      have a3: "\<And>n. n < length (map (interval_map real) I) \<Longrightarrow> x ! n \<in> set_of (map (interval_map real) I ! n)"
-        using 1(2) by simp
-        
-      have b1: "Ipoly x p1 \<in> set_of (Ipoly I (poly_map interval_of p1))"
-        using Ipoly_interval_args_mono[OF a1 a2 a3] t1_def(3)
-        by (simp add: Ipoly_real_float_interval_eqiv')
-      have b2: "Ipoly x p2 \<in> set_of (Ipoly I (poly_map interval_of p2))"
-        using Ipoly_interval_args_mono[OF a1 a2' a3] t2_def(3)
-        by (simp add: Ipoly_real_float_interval_eqiv')
-      
-      have "(f * g) x = f x * g x"
-        by auto
-      also have "... = (d1 + Ipoly x p1) * (d2 + Ipoly x p2)"
-        by (simp add: d1_def(2)[symmetric] d2_def(2)[symmetric])
-      also have "... = Ipoly x p1 * Ipoly x p2 + d1 * Ipoly x p2 + Ipoly x p1 * d2 + d1 * d2"
-        by (simp add: algebra_simps)
-      finally have f_times_g_eq: "(f * g) x - Ipoly x p1 * Ipoly x p2 = d1 * Ipoly x p2 + Ipoly x p1 * d2 + d1 * d2"
-        by simp
-      also have "... \<in> set_of (interval_map real (i1 * Ipoly I (poly_map interval_of p2))) +  set_of (interval_map real (Ipoly I (poly_map interval_of p1) * i2)) + set_of (i1 * i2)"
-        apply(rule set_plus_intro[OF set_plus_intro])
-        using d1_def(1) d2_def(1) b1 b2
-        by (simp_all add: set_of_mult_mono)
-      also have "... = set_of (interval_map real (i1 * Ipoly I (poly_map interval_of p2) + Ipoly I (poly_map interval_of p1) * i2 + i1 * i2))"
-        by (simp add: v1 v2 t1_def(2) t2_def(2) set_of_add_distrib valid_ivl_add)
-      finally have "(f * g) x - Ipoly x p1 * Ipoly x p2  \<in> set_of (interval_map real (i1 * Ipoly I (poly_map interval_of p2) + Ipoly I (poly_map interval_of p1) * i2 + i1 * i2))"
-        .
-
-      thus ?case
-      by simp
-    next
-      case 2
-      show ?case
-        using t1_def(2) t2_def(2) v1 v2
-        by (simp add: valid_ivl_add)
-    qed
-qed
-
-(* Taylor models for basic functions. *)
+lemma tm_id_valid:
+assumes "n < length I"
+shows "valid_tm I (interpret_floatarith (Var n)) (tm_id n)"
+using assms by simp
 
 (* Compute the nth derivative of a floatarith expression *)
 fun deriv :: "nat \<Rightarrow> floatarith \<Rightarrow> nat \<Rightarrow> floatarith"
@@ -668,19 +512,19 @@ by (simp_all add: valid_ivl_horner_eval)
 
 (* The interval coefficients of the taylor polynom,
    i.e. the real coefficients approximated by a float interval. *)
-fun TMf_c :: "nat \<Rightarrow> float interval \<Rightarrow> floatarith \<Rightarrow> float interval option"
-where "TMf_c n i f = compute_bound (Mult (deriv 0 f n) (Inverse (Num (fact n)))) [i]"
+fun tmf_c :: "nat \<Rightarrow> float interval \<Rightarrow> floatarith \<Rightarrow> float interval option"
+where "tmf_c n i f = compute_bound (Mult (deriv 0 f n) (Inverse (Num (fact n)))) [i]"
 
 (* Make a list of the n coefficients. *) 
-fun TMf_cs' :: "nat \<Rightarrow> float interval \<Rightarrow> float \<Rightarrow> floatarith \<Rightarrow> float interval option list"
-where "TMf_cs' 0 I a f = []"
-    | "TMf_cs' (Suc n) I a f = (TMf_c n (interval_of a) f) # (TMf_cs' n I a f)"
+fun tmf_cs' :: "nat \<Rightarrow> float interval \<Rightarrow> float \<Rightarrow> floatarith \<Rightarrow> float interval option list"
+where "tmf_cs' 0 I a f = []"
+    | "tmf_cs' (Suc n) I a f = (tmf_c n (interval_of a) f) # (tmf_cs' n I a f)"
 
 (* Also add the n+1-th coefficient, representing the error contribution, and reorder the list. *)
-fun TMf_cs :: "nat \<Rightarrow> float interval \<Rightarrow> float \<Rightarrow> floatarith \<Rightarrow> float interval list option"
-where "TMf_cs n I a f = those (rev (TMf_c n I f # (TMf_cs' n I a f)))"
+fun tmf_cs :: "nat \<Rightarrow> float interval \<Rightarrow> float \<Rightarrow> floatarith \<Rightarrow> float interval list option"
+where "tmf_cs n I a f = those (rev (tmf_c n I f # (tmf_cs' n I a f)))"
 
-value "the (TMf_cs 5 (Ivl 0 2) 1 (Cos (Var 0)))" 
+value "the (tmf_cs 5 (Ivl 0 2) 1 (Cos (Var 0)))" 
 
 (* TODO: Is this necessary? *)
 lemma of_nat_real_float_equiv: "(of_nat n :: real) = (of_nat n :: float)"
@@ -689,17 +533,17 @@ lemma of_nat_real_float_equiv: "(of_nat n :: real) = (of_nat n :: float)"
 lemma fact_real_float_equiv: "(fact n :: float) = (fact n :: real)"
   by (induction n, simp_all add: of_nat_real_float_equiv)
 
-lemma TMf_c_correct:
+lemma tmf_c_correct:
 fixes A::"float interval" and I::"float interval" and f::floatarith and a::real
 assumes "a \<in> set_of A"
-assumes "Some I = TMf_c i A f"
+assumes "Some I = tmf_c i A f"
 shows "valid_ivl I"
 and   "interpret_floatarith (deriv 0 f i) [a] / fact i \<in> set_of I"
 proof-
   obtain l u where I_decomp: "I = Ivl l u" using interval.exhaust by auto
 
   show result: "interpret_floatarith (deriv 0 f i) [a] / fact i \<in> set_of (interval_map real I)"
-    using compute_bound_correct[OF assms(2)[unfolded TMf_c.simps], where i="[a]"] assms(1)
+    using compute_bound_correct[OF assms(2)[unfolded tmf_c.simps], where i="[a]"] assms(1)
     by (simp add: divide_real_def fact_real_float_equiv)
   hence "set_of (interval_map real I) \<noteq> {}"
     by auto
@@ -765,92 +609,92 @@ proof-
     by (simp add: y_def)
 qed
 
-lemma TMf_cs_length:
-assumes "Some cs = TMf_cs n A a f"
+lemma tmf_cs_length:
+assumes "Some cs = tmf_cs n A a f"
 shows "length cs = n + 1"
-apply(simp add: Some_those_length[OF assms[unfolded TMf_cs.simps]])
+apply(simp add: Some_those_length[OF assms[unfolded tmf_cs.simps]])
 by (induction n, simp_all)
 
-lemma TMf_cs_correct:
+lemma tmf_cs_correct:
 fixes A::"float interval" and f::floatarith
 assumes "a \<in> set_of A"
-assumes "Some cs = TMf_cs n A a f"
-shows "\<And>i. i < n \<Longrightarrow> Some (cs!i) = TMf_c i (interval_of a) f"
-and   "Some (cs!n) = TMf_c n A f"
+assumes "Some cs = tmf_cs n A a f"
+shows "\<And>i. i < n \<Longrightarrow> Some (cs!i) = tmf_c i (interval_of a) f"
+and   "Some (cs!n) = tmf_c n A f"
 proof-
-  from TMf_cs_length[OF assms(2)]
+  from tmf_cs_length[OF assms(2)]
   have n_ineq: "n < length cs"
     by simp
-  from TMf_cs_length[OF assms(2)] assms(2)
-  have total_length: "length (TMf_c n A f # TMf_cs' n A a f) = Suc n"
-    by (metis Some_those_length Suc_eq_plus1 TMf_cs.simps length_rev)
+  from tmf_cs_length[OF assms(2)] assms(2)
+  have total_length: "length (tmf_c n A f # tmf_cs' n A a f) = Suc n"
+    by (metis Some_those_length Suc_eq_plus1 tmf_cs.simps length_rev)
     
-  from Some_those_nth[OF assms(2)[unfolded TMf_cs.simps] n_ineq]
-  show "Some (cs ! n) = TMf_c n A f"
+  from Some_those_nth[OF assms(2)[unfolded tmf_cs.simps] n_ineq]
+  show "Some (cs ! n) = tmf_c n A f"
     apply(subst (asm) rev_nth)
     using total_length by auto
 next
   fix i assume "i < n"
-  from TMf_cs_length[OF assms(2)] this
+  from tmf_cs_length[OF assms(2)] this
   have i_ineq: "i < length cs"
     by simp
 
-  from TMf_cs_length[OF assms(2)] assms(2)
-  have total_length: "length (TMf_c n A f # TMf_cs' n A a f) = Suc n"
-    by (metis Some_those_length Suc_eq_plus1 TMf_cs.simps length_rev)
+  from tmf_cs_length[OF assms(2)] assms(2)
+  have total_length: "length (tmf_c n A f # tmf_cs' n A a f) = Suc n"
+    by (metis Some_those_length Suc_eq_plus1 tmf_cs.simps length_rev)
     
-  have "Some (cs ! i) = (TMf_c n A f # TMf_cs' n A a f) ! (n - i)"
-    using Some_those_nth[OF assms(2)[unfolded TMf_cs.simps] i_ineq]
+  have "Some (cs ! i) = (tmf_c n A f # tmf_cs' n A a f) ! (n - i)"
+    using Some_those_nth[OF assms(2)[unfolded tmf_cs.simps] i_ineq]
     apply(subst (asm) rev_nth)
     using total_length `i < n`
     by auto
-  also have "... = (TMf_cs' n A a f) ! (n - Suc i)"
+  also have "... = (tmf_cs' n A a f) ! (n - Suc i)"
     using `i < n` by simp
-  also have "...  = TMf_c i (interval_of a) f"
+  also have "...  = tmf_c i (interval_of a) f"
     using `i < n` by (induction n, auto simp: less_Suc_eq)
-  finally show "Some (cs ! i) = TMf_c i (interval_of a) f" .
+  finally show "Some (cs ! i) = tmf_c i (interval_of a) f" .
 qed
 
-lemma TMf_cs_valid:
+lemma tmf_cs_valid:
 fixes A::"float interval" and f::floatarith
 assumes "a \<in> set_of A"
-assumes "Some cs = TMf_cs n A a f"
+assumes "Some cs = tmf_cs n A a f"
 shows "\<And>i. i \<le> n \<Longrightarrow> valid_ivl (cs!i)"
-using TMf_c_correct(1)[OF _ TMf_cs_correct(1)[OF assms], where a=a, simplified] 
-      TMf_c_correct(1)[OF _ TMf_cs_correct(2)[OF assms], where a=a, simplified, OF assms(1)]
+using tmf_c_correct(1)[OF _ tmf_cs_correct(1)[OF assms], where a=a, simplified] 
+      tmf_c_correct(1)[OF _ tmf_cs_correct(2)[OF assms], where a=a, simplified, OF assms(1)]
 by (auto simp: nat_less_le)
 
 
 abbreviation "x_minus_a\<equiv>\<lambda>a. poly.Sub (poly.Bound 0) (poly.C a)"
 
-fun TMfloatarith' :: "float \<Rightarrow> float interval list \<Rightarrow> float poly \<times> float interval poly"
-where "TMfloatarith' a [] = (poly.C 0, poly.C 0)"
-    | "TMfloatarith' a (c # cs) = (\<lambda>(pf, pi). (poly.Add (poly.C (mid c)) (poly.Mul (x_minus_a a) pf), poly.Add (poly.C (centered c)) (poly.Mul (x_minus_a (interval_of a)) pi))) (TMfloatarith' a cs)"
+fun tm_floatarith' :: "float \<Rightarrow> float interval list \<Rightarrow> float poly \<times> float interval poly"
+where "tm_floatarith' a [] = (poly.C 0, poly.C 0)"
+    | "tm_floatarith' a (c # cs) = (\<lambda>(pf, pi). (poly.Add (poly.C (mid c)) (poly.Mul (x_minus_a a) pf), poly.Add (poly.C (centered c)) (poly.Mul (x_minus_a (interval_of a)) pi))) (tm_floatarith' a cs)"
     
-fun TMfloatarith :: "nat \<Rightarrow> float interval \<Rightarrow> float \<Rightarrow> floatarith \<Rightarrow> taylor_model option"
-where "TMfloatarith n I a f = map_option (\<lambda>(pf, pi). TaylorModel pf (Ipoly [I] pi)) (map_option (TMfloatarith' a) (TMf_cs n I a f))"
+fun tm_floatarith :: "nat \<Rightarrow> float interval \<Rightarrow> float \<Rightarrow> floatarith \<Rightarrow> taylor_model option"
+where "tm_floatarith n I a f = map_option (\<lambda>(pf, pi). TaylorModel pf (Ipoly [I] pi)) (map_option (tm_floatarith' a) (tmf_cs n I a f))"
 
-value "TMfloatarith 5 (Ivl (-1) 1) 0 (Cos (Var 0))"
-value "interval_map real (compute_bound_tm (the (TMfloatarith 5 (Ivl (-1) 1) 0 (Cos (Var 0)))) [Ivl (-1) 1])"
+value "tm_floatarith 5 (Ivl (-1) 1) 0 (Cos (Var 0))"
+value "interval_map real (compute_bound_tm (the (tm_floatarith 5 (Ivl (-1) 1) 0 (Cos (Var 0)))) [Ivl (-1) 1])"
 
-lemma TMfloatarith_valid:
+lemma tm_floatarith_valid:
 assumes "0 < n"
 assumes "a \<in> set_of I"
 assumes "\<And>x. x \<in> set_of I \<Longrightarrow> isDERIV 0 f [x]"
-assumes "Some t = TMfloatarith n I a f"
+assumes "Some t = tm_floatarith n I a f"
 shows "valid_tm [I] (interpret_floatarith f) t"
 proof-
-  from assms(4)[unfolded TMfloatarith.simps]
-  obtain pf pi where Some_pf_pi_def: "Some (pf, pi) = map_option (TMfloatarith' a) (TMf_cs n I a f)"
+  from assms(4)[unfolded tm_floatarith.simps]
+  obtain pf pi where Some_pf_pi_def: "Some (pf, pi) = map_option (tm_floatarith' a) (tmf_cs n I a f)"
     by (metis (no_types, lifting) map_option_eq_Some prod.collapse)
   then have t_def: "t = TaylorModel pf (Ipoly [I] pi)"
-    using assms(4)[unfolded TMfloatarith.simps]
+    using assms(4)[unfolded tm_floatarith.simps]
     by (metis old.prod.case option.sel option.simps(9))
-  from Some_pf_pi_def obtain cs where cs_def: "Some cs = TMf_cs n I a f"
+  from Some_pf_pi_def obtain cs where cs_def: "Some cs = tmf_cs n I a f"
     by (metis map_option_eq_Some)
-  have pfpi_def: "(pf, pi) = TMfloatarith' a cs"
+  have pfpi_def: "(pf, pi) = tm_floatarith' a cs"
     by (metis Some_pf_pi_def cs_def map_option_eq_Some option.sel)
-  from TMf_cs_valid[OF assms(2) cs_def] TMf_cs_length[OF cs_def]
+  from tmf_cs_valid[OF assms(2) cs_def] tmf_cs_length[OF cs_def]
   have valid_cs: "\<And>i. i < length cs \<Longrightarrow> valid_ivl (cs ! i)"
     by auto
   
@@ -865,7 +709,7 @@ proof-
       apply(simp add: zero_interval_def)
       proof-
         case (Cons c cs pf pi)
-        then obtain pf' pi' where pf'pi'_def: "(pf', pi') = TMfloatarith' a cs"
+        then obtain pf' pi' where pf'pi'_def: "(pf', pi') = tm_floatarith' a cs"
           using prod.collapse by blast
         from this Cons(2)[simplified]
         have pi_decomp: "pi = poly.Add (c - Ivl (mid c) (mid c))\<^sub>p (Mul (x_minus_a (Ivl a a)) pi')"
@@ -880,7 +724,7 @@ proof-
       apply(simp)
       proof-
         case (Cons c cs pf pi)
-        then obtain pf' pi' where pf'pi'_def: "(pf', pi') = TMfloatarith' a cs"
+        then obtain pf' pi' where pf'pi'_def: "(pf', pi') = tm_floatarith' a cs"
           using prod.collapse by blast
         from this Cons(2)[simplified]
         have pf_decomp: "pf = poly.Add (mid c)\<^sub>p (Mul (x_minus_a a) pf')"
@@ -898,12 +742,12 @@ proof-
     proof(cases "x = a")
       case True
       have pf_val_at_a: "Ipoly [real a] (poly_map real pf) = mid (cs ! 0)"
-        using pfpi_def TMf_cs_length[OF cs_def]
+        using pfpi_def tmf_cs_length[OF cs_def]
         apply(induction cs arbitrary: pf pi n)
         apply(simp)
         proof-
           case (Cons c cs pf pi n)
-          then obtain pf' pi' where pf'pi'_def: "(pf', pi') = TMfloatarith' a cs"
+          then obtain pf' pi' where pf'pi'_def: "(pf', pi') = tm_floatarith' a cs"
             using prod.collapse by blast
           from this Cons(2)[simplified]
           have pf_decomp: "pf = poly.Add (mid c)\<^sub>p (Mul (x_minus_a a) pf')"
@@ -912,15 +756,15 @@ proof-
             using Cons(1)[OF pf'pi'_def]
             by (simp add: pf_decomp)
         qed
-      from TMf_c_correct(2)[OF _ TMf_cs_correct(1)[OF assms(2) cs_def assms(1)], of a]
+      from tmf_c_correct(2)[OF _ tmf_cs_correct(1)[OF assms(2) cs_def assms(1)], of a]
       have "interpret_floatarith f xs \<in> set_of (interval_map real (cs ! 0))"
         by (simp add: xs_def `x = a`)
       have "interpret_floatarith f xs - Ipoly xs (poly_map real pf) \<in> set_of (interval_map real (cs ! 0) - (mid (cs ! 0)))"
-        using pf_val_at_a TMf_c_correct(2)[OF _ TMf_cs_correct(1)[OF assms(2) cs_def assms(1)], of a]
+        using pf_val_at_a tmf_c_correct(2)[OF _ tmf_cs_correct(1)[OF assms(2) cs_def assms(1)], of a]
         by (simp add: xs_def `x = a` set_of_minus_mono)
       also have "... \<subseteq>  set_of (interval_map real (Ipoly [I] pi))"
         proof-
-          from TMf_cs_length[OF cs_def]
+          from tmf_cs_length[OF cs_def]
           obtain c cs' where cs_decomp: "cs = c # cs'" 
             by (metis Suc_eq_plus1 list.size(3) neq_Nil_conv old.nat.distinct(2))
           obtain pi' where pi_decomp: "pi = poly.Add (c - interval_of (mid c))\<^sub>p (Mul (x_minus_a (interval_of a)) pi')"
@@ -930,7 +774,7 @@ proof-
           show ?thesis
             apply(simp add: cs_decomp pi_decomp)
             apply(rule set_of_add_inc[where B=0, simplified])
-            using valid_cs[of 0] TMf_cs_length[OF cs_def]
+            using valid_cs[of 0] tmf_cs_length[OF cs_def]
             apply(simp add: valid_ivl_sub cs_decomp)
             apply(simp add: zero_interval_def)
             apply(simp)
@@ -969,13 +813,13 @@ proof-
         apply(simp add: I_def)
         by (meson less_eq_real_def order_trans)
       
-      from pfpi_def TMf_cs_length[OF cs_def]
+      from pfpi_def tmf_cs_length[OF cs_def]
       have Ipoly_pf_eq: "Ipoly xs pf = (\<Sum>m<Suc n. mid (cs!m) * (x - a) ^ m)"
         apply(induction cs arbitrary: n pf pi)
         apply(simp add: xs_def)
         proof-
           case (Cons c cs n pf pi)
-          obtain pf' pi' where pf'pi'_def: "(pf', pi') = TMfloatarith' a cs"
+          obtain pf' pi' where pf'pi'_def: "(pf', pi') = tm_floatarith' a cs"
             using prod.collapse by blast
           from Cons(2)
           have pf_def: "pf = poly.Add (mid c)\<^sub>p (Mul (x_minus_a a) pf')"
@@ -1027,10 +871,10 @@ proof-
         apply(rule horner_eval_interval)
         apply(simp add: cr_def ci_def)
         apply(safe)[1]
-        using TMf_c_correct(2)[OF _ TMf_cs_correct(1)[OF  assms(2) cs_def], where a=a, simplified]
+        using tmf_c_correct(2)[OF _ tmf_cs_correct(1)[OF  assms(2) cs_def], where a=a, simplified]
         apply(simp)
         apply(rule set_of_minus_mono)
-        using TMf_c_correct(2)[OF t_in_I TMf_cs_correct(2)[OF assms(2) cs_def]]
+        using tmf_c_correct(2)[OF t_in_I tmf_cs_correct(2)[OF assms(2) cs_def]]
         apply(simp_all)
         proof(goals)
           case(1 i)
@@ -1041,7 +885,7 @@ proof-
             by simp
         qed
       also have "... \<subseteq> set_of (interval_map real (Ipoly [I] pi))"
-        using ci_def pfpi_def TMf_cs_length[OF cs_def] valid_cs
+        using ci_def pfpi_def tmf_cs_length[OF cs_def] valid_cs
         proof(induction n arbitrary: cs pi pf ci)
           case (0 cs pi pf)
           from 0(2) obtain c where cs_def: "cs = [c]"
@@ -1056,7 +900,7 @@ proof-
                                    and length_cs': "length cs' = n + 1"
             by (metis Suc_eq_plus1 length_Suc_conv)
           hence "cs' \<noteq> []" by auto
-          from cs_def obtain pf' pi' where pf'pi'_def: "(pf', pi') = TMfloatarith' a cs'"
+          from cs_def obtain pf' pi' where pf'pi'_def: "(pf', pi') = tm_floatarith' a cs'"
             using prod.collapse by blast
           from Suc(2) have pi_def: "pi = poly.Add (centered c)\<^sub>p (Mul (x_minus_a (Ivl a a)) pi')"
             by (simp add: cs_def pf'pi'_def[symmetric])
@@ -1094,63 +938,348 @@ qed
 definition Sin::"floatarith \<Rightarrow> floatarith"
 where "Sin a = Minus (Cos (Add (Mult Pi (Num (Float 1 (- 1)))) (Minus a)))"
 
+(* Operations on taylor models. *)
+fun tm_neg :: "taylor_model \<Rightarrow> taylor_model"
+where "tm_neg (TaylorModel p i) = TaylorModel (poly.Neg p) (-i)"
+
+fun tm_add :: "taylor_model \<Rightarrow> taylor_model \<Rightarrow> taylor_model"
+where "tm_add (TaylorModel p1 i1) (TaylorModel p2 i2) = TaylorModel (poly.Add p1 p2) (i1+i2)"
+
+fun tm_sub :: "taylor_model \<Rightarrow> taylor_model \<Rightarrow> taylor_model"
+where "tm_sub t1 t2 = tm_add t1 (tm_neg t2)"
+
+(* TODO: Currently, this increases the degree of the polynomial! *)
+fun tm_mul :: "taylor_model \<Rightarrow> taylor_model \<Rightarrow> float interval list \<Rightarrow> taylor_model"
+where "tm_mul (TaylorModel p1 i1) (TaylorModel p2 i2) I = (
+  let d1=Ipoly I p1;
+      d2=Ipoly I p2
+  in TaylorModel (poly.Mul p1 p2) (i1*d2 + d1*i2 + i1*i2))"
+  
+fun tm_pow :: "taylor_model \<Rightarrow> nat \<Rightarrow> float interval list \<Rightarrow> taylor_model"
+where "tm_pow t 0 I = TaylorModel (poly.C 1) (Ivl 0 0)"
+    | "tm_pow t (Suc n) I = tm_mul t (tm_pow t n I) I"
+
+fun tm_inc_error :: "taylor_model \<Rightarrow> float interval \<Rightarrow> taylor_model"
+where "tm_inc_error (TaylorModel p e) i = TaylorModel p (e+i)"
+
+(*
+datatype 'a poly = C 'a | Bound nat | Add "'a poly" "'a poly" | Sub "'a poly" "'a poly"
+  | Mul "'a poly" "'a poly"| Neg "'a poly"| Pw "'a poly" nat | CN "'a poly" nat "'a poly"
+*)
+(* Evaluates a float polynomial, using a taylor model as the parameter. This is used to compose taylor models. *)
+fun eval_poly_at_tm :: "float poly \<Rightarrow> taylor_model \<Rightarrow> float interval list \<Rightarrow> taylor_model"
+where "eval_poly_at_tm (poly.C c) t I = tm_const c"
+    | "eval_poly_at_tm (poly.Bound n) t I = (if n = 0 then t else undefined)"
+    | "eval_poly_at_tm (poly.Add p1 p2) t I = tm_add (eval_poly_at_tm p1 t I) (eval_poly_at_tm p2 t I)"
+    | "eval_poly_at_tm (poly.Sub p1 p2) t I = tm_sub (eval_poly_at_tm p1 t I) (eval_poly_at_tm p2 t I)"
+    | "eval_poly_at_tm (poly.Mul p1 p2) t I = tm_mul (eval_poly_at_tm p1 t I) (eval_poly_at_tm p2 t I) I"
+    | "eval_poly_at_tm (poly.Neg p) t I = tm_neg (eval_poly_at_tm p t I)"
+    | "eval_poly_at_tm (poly.Pw p n) t I = tm_pow (eval_poly_at_tm p t I) n I"
+    | "eval_poly_at_tm (poly.CN c n p) t I = tm_add (eval_poly_at_tm c t I) (tm_mul (if n = 0 then t else undefined) (eval_poly_at_tm p t I) I)"
+
+fun tm_comp :: "taylor_model \<Rightarrow> taylor_model \<Rightarrow> float interval list \<Rightarrow> taylor_model"
+where "tm_comp (TaylorModel p e) t I = tm_inc_error (eval_poly_at_tm p t I) e"
+
+(* Validity of is preserved under taylor model arithmetic. *)
+lemma tm_neg_valid:
+assumes "valid_tm I f t"
+shows "valid_tm I (-f) (tm_neg t)"
+proof-
+  from valid_tmD[OF assms]
+  obtain p l u where t_def: 
+    "t = TaylorModel p (Ivl l u)"
+    "valid_ivl (Ivl l u)"
+    "num_params p \<le> length I"
+    "\<And>x. length x = length I \<Longrightarrow> (\<And>n. n < length I \<Longrightarrow> x ! n \<in> set_of (interval_map real (I ! n))) \<Longrightarrow> f x - Ipoly x p \<in> {l..u}"
+      by blast
+  show ?thesis
+    apply(rule)
+    apply(simp add: t_def(1) uminus_interval_def)
+    using t_def(2)
+    apply(simp)
+    apply(simp add: t_def(3))
+    proof-
+      fix x assume assms: "length x = length I" "(\<And>n. n < length I \<Longrightarrow> x ! n \<in> set_of (interval_map real (I ! n)))"
+      show "(-f) x - Ipoly x (Neg p) \<in> {(-u)..(-l)}"
+        using t_def(4)[OF assms] by simp
+    qed
+qed
+
+lemma tm_add_valid:
+assumes "valid_tm I f t1"
+assumes "valid_tm I g t2"
+shows "valid_tm I (f + g) (tm_add t1 t2)"
+proof-
+  from valid_tmD[OF assms(1)]
+  obtain p1 l1 u1 where t1_def:
+    "t1 = TaylorModel p1 (Ivl l1 u1)"
+    "valid_ivl (Ivl l1 u1)"
+    "num_params p1 \<le> length I"
+    "\<And>x. length x = length I \<Longrightarrow> (\<And>n. n < length I \<Longrightarrow> x ! n \<in> set_of (interval_map real (I ! n))) \<Longrightarrow> f x - Ipoly x p1 \<in> {l1..u1}"
+      by blast
+  from valid_tmD[OF assms(2)]
+  obtain p2 l2 u2 where t2_def:
+    "t2 = TaylorModel p2 (Ivl l2 u2)"
+    "valid_ivl (Ivl l2 u2)"
+    "num_params p2 \<le> length I"
+    "\<And>x. length x = length I \<Longrightarrow> (\<And>n. n < length I \<Longrightarrow> x ! n \<in> set_of (interval_map real (I ! n))) \<Longrightarrow> g x - Ipoly x p2 \<in> {l2..u2}"
+      by blast
+   
+  show "valid_tm I (f + g) (tm_add t1 t2)"
+    proof(rule)
+      show "num_params (poly.Add p1 p2) \<le> length I"
+      by (simp add: t1_def(3) t2_def(3))
+    next
+      fix x assume assms: "length x = length I" "(\<And>n. n < length I \<Longrightarrow> x ! n \<in> set_of (interval_map real (I ! n)))"
+      from t1_def(4)[OF this] t2_def(4)[OF this]
+       show "(f + g) x - Ipoly x (poly.Add p1 p2) \<in> {(l1+l2)..(u1+u2)}"
+        by simp
+    next
+      show "valid_ivl (Ivl (l1 + l2) (u1 + u2))"
+        using t1_def(2) t2_def(2)
+        by simp
+    qed (simp add: t1_def(1) t2_def(1) plus_interval_def)
+qed
+
+lemma tm_sub_valid:
+assumes "valid_tm I f t1"
+assumes "valid_tm I g t2"
+shows "valid_tm I (f - g) (tm_sub t1 t2)"
+using tm_add_valid[OF assms(1) tm_neg_valid[OF assms(2)]]
+by simp
+
+(* TODO: Clean this proof up! *)
+lemma tm_mul_valid:
+assumes "valid_tm I f t1"
+assumes "valid_tm I g t2"
+assumes "\<And>n. n < length I \<Longrightarrow> valid_ivl (I ! n)" (* TODO: Should validity of I be part of valid_tm? *)
+shows "valid_tm I (f * g) (tm_mul t1 t2 I)"
+proof-
+  from valid_tmD'[OF assms(1)]
+  obtain p1 i1 where t1_def:
+    "t1 = TaylorModel p1 i1"
+    "valid_ivl i1"
+    "num_params p1 \<le> length I"
+    "\<And>x. length x = length I \<Longrightarrow> (\<And>n. n < length I \<Longrightarrow> x ! n \<in> set_of (interval_map real (I ! n))) \<Longrightarrow> f x - Ipoly x p1 \<in> set_of i1"
+      by blast
+  from valid_tmD'[OF assms(2)]
+  obtain p2 i2 where t2_def:
+    "t2 = TaylorModel p2 i2"
+    "valid_ivl i2"
+    "num_params p2 \<le> length I"
+    "\<And>x. length x = length I \<Longrightarrow> (\<And>n. n < length I \<Longrightarrow> x ! n \<in> set_of (interval_map real (I ! n))) \<Longrightarrow> g x - Ipoly x p2 \<in> set_of i2"
+      by blast
+        
+  have v1: "valid_ivl (Ipoly I (poly_map interval_of p1))"
+    by (rule valid_ivl_Ipoly[OF t1_def(3) assms(3)])
+  have v2: "valid_ivl (Ipoly I (poly_map interval_of p2))"
+    by (rule valid_ivl_Ipoly[OF t2_def(3) assms(3)])
+      
+  show "valid_tm I (f * g) (tm_mul t1 t2 I)"
+    unfolding t1_def t2_def tm_mul.simps Let_def
+    apply(rule valid_tmI')
+    unfolding taylor_model.inject
+    apply(rule conjI[OF refl refl])
+    defer
+    using t1_def(3) t2_def(3)
+    apply(simp)
+    proof(goals)
+      case (1 x)
+      
+      obtain d1 :: real where d1_def: "d1 \<in> set_of i1" "f x - Ipoly x p1 = d1"
+        using t1_def(4)[OF 1] by auto
+      obtain d2 :: real where d2_def: "d2 \<in> set_of i2" "g x - Ipoly x p2 = d2"
+        using t2_def(4)[OF 1] by auto
+        
+      have a1: "length x = length (map (interval_map real) I)"
+        using 1(1) by simp
+      have a2: "num_params (poly_map real p1) \<le> length (map (interval_map real) I)"
+        using t1_def(3) by simp
+      have a2': "num_params (poly_map real p2) \<le> length (map (interval_map real) I)"
+        using t2_def(3) by simp
+      have a3: "\<And>n. n < length (map (interval_map real) I) \<Longrightarrow> x ! n \<in> set_of (map (interval_map real) I ! n)"
+        using 1(2) by simp
+        
+      have b1: "Ipoly x p1 \<in> set_of (Ipoly I (poly_map interval_of p1))"
+        using Ipoly_interval_args_mono[OF a1 a2 a3] t1_def(3)
+        by (simp add: Ipoly_real_float_interval_eqiv')
+      have b2: "Ipoly x p2 \<in> set_of (Ipoly I (poly_map interval_of p2))"
+        using Ipoly_interval_args_mono[OF a1 a2' a3] t2_def(3)
+        by (simp add: Ipoly_real_float_interval_eqiv')
+      
+      have "(f * g) x = f x * g x"
+        by auto
+      also have "... = (d1 + Ipoly x p1) * (d2 + Ipoly x p2)"
+        by (simp add: d1_def(2)[symmetric] d2_def(2)[symmetric])
+      also have "... = Ipoly x p1 * Ipoly x p2 + d1 * Ipoly x p2 + Ipoly x p1 * d2 + d1 * d2"
+        by (simp add: algebra_simps)
+      finally have f_times_g_eq: "(f * g) x - Ipoly x p1 * Ipoly x p2 = d1 * Ipoly x p2 + Ipoly x p1 * d2 + d1 * d2"
+        by simp
+      also have "... \<in> set_of (interval_map real (i1 * Ipoly I (poly_map interval_of p2))) +  set_of (interval_map real (Ipoly I (poly_map interval_of p1) * i2)) + set_of (i1 * i2)"
+        apply(rule set_plus_intro[OF set_plus_intro])
+        using d1_def(1) d2_def(1) b1 b2
+        by (simp_all add: set_of_mult_mono)
+      also have "... = set_of (interval_map real (i1 * Ipoly I (poly_map interval_of p2) + Ipoly I (poly_map interval_of p1) * i2 + i1 * i2))"
+        by (simp add: v1 v2 t1_def(2) t2_def(2) set_of_add_distrib valid_ivl_add)
+      finally have "(f * g) x - Ipoly x p1 * Ipoly x p2  \<in> set_of (interval_map real (i1 * Ipoly I (poly_map interval_of p2) + Ipoly I (poly_map interval_of p1) * i2 + i1 * i2))"
+        .
+
+      thus ?case
+      by simp
+    next
+      case 2
+      show ?case
+        using t1_def(2) t2_def(2) v1 v2
+        by (simp add: valid_ivl_add)
+    qed
+qed
+
+lemma tm_pow_valid:
+assumes "valid_tm I f t"
+assumes "\<And>n. n < length I \<Longrightarrow> valid_ivl (I ! n)"
+shows "valid_tm I (f ^ n) (tm_pow t n I)"
+apply(induction n, simp)
+using assms(1) tm_mul_valid[OF _ _ assms(2)]
+by force
+
+lemma fun_pow: "f^n = (\<lambda>x. (f x)^n)"
+by (induction n, simp_all)
+        
+lemma tm_comp_valid:
+assumes I_valid: "(\<And>n. n < length I \<Longrightarrow> valid_ivl (I ! n))"
+assumes gI_def: "\<And>x. length x = length I \<Longrightarrow> (\<forall>n<length I. x!n \<in> set_of (I!n)) \<Longrightarrow> g x \<in> set_of gI"
+assumes t1_def: "valid_tm [gI] (\<lambda>x. f (hd x)) t1"
+assumes t2_def: "valid_tm I g t2"
+shows "valid_tm I (f o g) (tm_comp t1 t2 I)"
+proof-
+  obtain pf ef where t1_decomp: "t1 = TaylorModel pf ef" using taylor_model.exhaust by auto
+  obtain pg eg where t2_decomp: "t2 = TaylorModel pg eg" using taylor_model.exhaust by auto
+  
+  from t1_def have t1_valid:
+    "valid_ivl ef"
+    "num_params pf \<le> 1"
+    "\<And>x. length x = length I \<Longrightarrow> \<forall>n<length I. x ! n \<in> set_of (interval_map real (I ! n))
+          \<Longrightarrow> f (g x) - Ipoly [g x] (poly_map real pf) \<in> set_of ef"
+      using gI_def
+      by (simp_all add: t1_decomp, metis length_Cons list.sel(1) list.size(3) nth_Cons_0)
+      
+  from t2_def have t2_valid:
+    "valid_ivl eg"
+    "num_params pg \<le> length I"
+    "\<And>x. length x = length I \<Longrightarrow> (\<forall>n<length I. x ! n \<in> set_of (interval_map real (I ! n))) 
+          \<Longrightarrow> g x - Ipoly x (poly_map real pg) \<in> set_of (interval_map real eg)"
+      by (auto simp: t2_decomp)
+      
+  obtain p' e' where p'e'_def: "TaylorModel p' e' = eval_poly_at_tm pf t2 I"
+    using taylor_model.exhaust by metis
+    
+  have "valid_tm I ((\<lambda>x. Ipoly [x] pf) o g) (eval_poly_at_tm pf t2 I)"
+    using t1_valid(2)
+    proof(induction pf)
+      case (C c) thus ?case
+        by simp
+    next
+      case (Bound n) thus ?case
+        by (simp add: t2_decomp t2_valid)
+    next
+      case (Add p1l p1r) thus ?case 
+        using tm_add_valid by (simp add: func_plus)
+    next
+      case (Sub p1l p1r) thus ?case 
+        using tm_sub_valid by (simp add: fun_diff_def)
+    next
+      case (Mul p1l p1r) thus ?case 
+        using tm_mul_valid[OF _ _ I_valid] by (simp add: func_times)
+    next
+      case (Neg p1') thus ?case 
+        using tm_neg_valid by (simp add: fun_Compl_def)
+    next
+      case (Pw p1' n) thus ?case 
+        using tm_pow_valid[OF _ I_valid] by (simp add: fun_pow)
+    next
+      case (CN p1l n p1r) thus ?case 
+        using tm_add_valid[OF _ tm_mul_valid[OF _ _ I_valid], unfolded func_plus func_times] t2_def by simp
+    qed
+     
+  hence eval_poly_at_tm_valid:
+    "valid_ivl e'"
+    "num_params p' \<le> length I"
+    "\<forall>x. length x = length I \<and> (\<forall>n<length I. x ! n \<in> set_of (interval_map real (I ! n))) \<longrightarrow>
+         Ipoly [g x] (poly_map real pf) - Ipoly x (poly_map real p') \<in> set_of (interval_map real e')"
+      by (auto simp: t1_decomp p'e'_def[symmetric])
+  show ?thesis
+    apply(simp add: t1_decomp p'e'_def[symmetric])
+    apply(safe)
+    apply(rule valid_ivl_add[OF eval_poly_at_tm_valid(1) t1_valid(1)])
+    using eval_poly_at_tm_valid(2)
+    apply(simp)
+    proof(goals)
+      case (1 x)
+      have "Ipoly [g x] (poly_map real pf) - Ipoly x (poly_map real p') \<in> set_of e'"
+        using 1 eval_poly_at_tm_valid(3)
+        by simp
+      thus ?case
+        using set_of_add_mono t1_valid(3)[OF 1]
+        by force
+    qed
+qed
+
 (* Compute taylor models of degree n from floatarith expressions.
    TODO: For now, this returns an option. This will change as soon as 
          all of floatarith can be converted to a taylor model. *)
-fun compute_taylor_model :: "nat \<Rightarrow> float interval list \<Rightarrow> floatarith \<Rightarrow> taylor_model option"
-where "compute_taylor_model _ I (Num c) = Some (TaylorModel (poly.C c) (Ivl 0 0))"
-    | "compute_taylor_model _ I (Var n) = Some (TaylorModel (poly.Bound n) (Ivl 0 0))"
-    | "compute_taylor_model n I (Add a b) = (
-         case (compute_taylor_model n I a, compute_taylor_model n I b) 
-         of (Some t1, Some t2) \<Rightarrow> Some (TMAdd t1 t2) | _ \<Rightarrow> None)"
-    | "compute_taylor_model n I (Minus a) = (
-         case compute_taylor_model n I a of Some t1 \<Rightarrow> Some (TMNeg t1) | _ \<Rightarrow> None)"
-    | "compute_taylor_model n I _ = None"
+fun compute_tm :: "nat \<Rightarrow> float interval list \<Rightarrow> floatarith \<Rightarrow> taylor_model option"
+where "compute_tm _ I (Num c) = Some (tm_const c)"
+    | "compute_tm _ I (Var n) = Some (tm_id n)"
+    | "compute_tm n I (Add a b) = (
+         case (compute_tm n I a, compute_tm n I b) 
+         of (Some t1, Some t2) \<Rightarrow> Some (tm_add t1 t2) | _ \<Rightarrow> None)"
+    | "compute_tm n I (Minus a) = map_option (\<lambda>t. tm_neg t) (compute_tm n I a)"
+    | "compute_tm n I _ = None"
 
-lemma computed_taylor_model_valid:
+lemma compute_tm_valid:
 assumes "num_vars f \<le> length I"
-assumes "Some t = compute_taylor_model n I f"
+assumes "Some t = compute_tm n I f"
 shows "valid_tm I (interpret_floatarith f) t"
 using assms
 proof(induct f arbitrary: t)
 case (Add a b t)
-  obtain t1 where t1_def: "Some t1 = compute_taylor_model n I a"
-    by (metis (no_types, lifting) Add(4) compute_taylor_model.simps(3) option.case_eq_if option.collapse prod.case)
-  obtain t2 where t2_def: "Some t2 = compute_taylor_model n I b"
-    by (smt Add(4) compute_taylor_model.simps(3) option.case_eq_if option.collapse prod.case)
-  have t_def: "t = TMAdd t1 t2"
+  obtain t1 where t1_def: "Some t1 = compute_tm n I a"
+    by (metis (no_types, lifting) Add(4) compute_tm.simps(3) option.case_eq_if option.collapse prod.case)
+  obtain t2 where t2_def: "Some t2 = compute_tm n I b"
+    by (smt Add(4) compute_tm.simps(3) option.case_eq_if option.collapse prod.case)
+  have t_def: "t = tm_add t1 t2"
     using Add(4) t1_def t2_def
-    by (metis compute_taylor_model.simps(3) option.case(2) option.inject prod.case)
+    by (metis compute_tm.simps(3) option.case(2) option.inject prod.case)
   
   have [simp]: "interpret_floatarith (floatarith.Add a b) = interpret_floatarith a + interpret_floatarith b"
     by auto
   show "valid_tm I (interpret_floatarith (floatarith.Add a b)) t"
     apply(simp add: t_def)
-    apply(rule TMAdd_valid[OF Add(1)[OF _ t1_def] Add(2)[OF _ t2_def]])
+    apply(rule tm_add_valid[OF Add(1)[OF _ t1_def] Add(2)[OF _ t2_def]])
     using Add(3) by auto
 next
 case (Minus a t)
    have [simp]: "interpret_floatarith (Minus a) = -interpret_floatarith a"
      by auto
    
-   obtain t1 where t1_def: "Some t1 = compute_taylor_model n I a"
-     by (metis Minus(3) compute_taylor_model.simps(4) option.collapse option.simps(4))
-   have t_def: "t = TMNeg t1"
-     by (metis Minus(3) compute_taylor_model.simps(4) option.case(2) option.inject t1_def)
+   obtain t1 where t1_def: "Some t1 = compute_tm n I a"
+     by (metis Minus.prems(2) compute_tm.simps(4) map_option_eq_Some)
+   have t_def: "t = tm_neg t1"
+     by (metis Minus.prems(2) compute_tm.simps(4) option.inject option.simps(9) t1_def)
      
    show "valid_tm I (interpret_floatarith (Minus a)) t"
-     apply(simp add: t_def, rule TMNeg_valid[OF Minus(1)[OF _ t1_def]])
+     apply(simp add: t_def, rule tm_neg_valid[OF Minus(1)[OF _ t1_def]])
      using Minus(2) by auto
 qed (simp_all add: valid_tm_def)
 
 (* Compute some taylor models. *)
-value "the (compute_taylor_model 10 [Ivl 0 1] (Num 2))"
-value "the (compute_taylor_model 10 [Ivl 0 1] (Var 0))"
-value "the (compute_taylor_model 10 [Ivl 0 1, Ivl 0 1] (Add (Var 0) (Var 1)))"
+value "the (compute_tm 10 [Ivl 0 1] (Num 2))"
+value "the (compute_tm 10 [Ivl 0 1] (Var 0))"
+value "the (compute_tm 10 [Ivl 0 1, Ivl 0 1] (Add (Var 0) (Var 1)))"
 
 (* Automatically find interval bounds for floatarith expressions. *)
 fun compute_ivl_bound :: "nat \<Rightarrow> float interval list \<Rightarrow> floatarith \<Rightarrow> float interval option"
-where "compute_ivl_bound n I f = (case compute_taylor_model n I f of None \<Rightarrow> None | Some t \<Rightarrow> Some (compute_bound_tm t I))"
+where "compute_ivl_bound n I f = (case compute_tm n I f of None \<Rightarrow> None | Some t \<Rightarrow> Some (compute_bound_tm t I))"
 
 (* Automatically computed bounds are correct. *)
 lemma compute_ivl_bound_correct:
@@ -1162,9 +1291,9 @@ shows "interpret_floatarith f x \<in> set_of B"
 proof-
   (* Since we have a bound B, there must have been a taylor model used to compute it. *)
   from assms(2) obtain t where B_def: "B = compute_bound_tm t I" 
-                           and t_def: "Some t = compute_taylor_model n I f"
+                           and t_def: "Some t = compute_tm n I f"
     by (simp, metis (mono_tags, lifting) option.case_eq_if option.collapse option.distinct(1) option.inject)
-  from compute_bound_tm_correct[OF computed_taylor_model_valid[OF assms(1) t_def] assms(3,4)]
+  from compute_bound_tm_correct[OF compute_tm_valid[OF assms(1) t_def] assms(3,4)]
   show ?thesis
     by (simp add: B_def)
 qed
